rwlock automation

dafny/code/RwLockDerivation.dfy
@@ -1,110 +1,162 @@
-include "HashTableDerivation.dfy"
-
 module RWLock {
-  /* Define the RwLock TPCM Extension */
+  /* Assume a type of object to be stored */
 
-  import Base = HashTable
+  type X
 
-  datatype CentralState = CentralState(
-    exc: bool,
-    rc: nat,
-    held_value: Base.M
-  ) | None
+  /* Auxilliary defs */
 
-  predicate IsFull<K(!new), V>(m: imap<K, V>) {
-    forall k :: k in m
+  datatype Exc<T> = ExcEmpty | ExcOne(t: T) | ExcFail
+
+  function exc_unit<T>(): Exc<T> {
+      ExcEmpty
   }
 
-  type FullMap<K(!new), V> = m : imap<K, V> | IsFull(m)
-    witness *
+  function exc_dot<T>(x: Exc<T>, y: Exc<T>): Exc<T> {
+      if x == ExcEmpty then y
+      else if y == ExcEmpty then x
+      else ExcFail
+  } 
+
+  predicate exc_valid<T>(x: Exc<T>) {
+      x != ExcFail
+  }
+
+  type positive_nat = n: nat | n >= 1 witness 1
+  datatype Agn<T> = Zero | Have(t: T, n: positive_nat) | AgnFail
+
+  function agn_unit<T>(): Agn<T> {
+      Zero
+  }
+
+  function agn_dot<T>(x: Agn<T>, y: Agn<T>): Agn<T> {
+      match x {
+          case Zero => y
+          case Have(tx, nx) => match y {
+              case Zero => x
+              case Have(ty, ny) => if tx == ty then Have(tx, nx + ny) else AgnFail
+              case AgnFail => AgnFail
+          }
+          case AgnFail => AgnFail
+      }
+  }
+
+  predicate agn_valid<T>(x: Agn<T>) {
+      x != AgnFail
+  }
+
+  /* The Base monoid */
+
+  type B = Exc<X>
+
+  function base_unit() : B {
+      exc_unit()
+  }
+
+  function base_dot(x: B, y: B) : B {
+      exc_dot(x, y)
+  }
+
+  predicate base_V(x: B) {
+      exc_valid(x)
+  }
+
+  lemma base_commutative(a: B, b: B)
+  ensures base_dot(a, b) == base_dot(b, a)
+  {
+  }
+
+  lemma base_associative(a: B, b: B, c: B)
+  ensures base_dot(a, base_dot(b, c)) == base_dot(base_dot(a, b), c)
+  {
+  }
+
+  lemma base_dot_unit(a: B)
+  ensures base_dot(a, base_unit()) == a
+  {
+  }
+
+  lemma base_valid_monotonic(a: B, b: B)
+  requires base_V(base_dot(a, b))
+  ensures base_V(a)
+  {
+  }
+
+  lemma base_valid_unit()
+  ensures base_V(base_unit())
+  {
+  }
+
+  /* Define the RwLock storage protocol */
+
+  datatype FieldsState = FieldsState(
+    exc: bool,
+    rc: int,
+    x: X
+  )
 
   datatype F = F(
-    central: CentralState,
-    exc_pending: bool,
-    exc_taken: bool,
+    fields: Exc<FieldsState>,
+    exc_pending: Exc<()>,
+    exc_taken: Exc<()>,
     shared_pending_handles: nat,
-    ghost shared_taken_handles: FullMap<Base.M, nat>
-  ) | Bot
-
-  function zero_map() : imap<Base.M, nat> {
-    imap k | true :: 0
-  }
+    shared_taken_handles: Agn<X>
+  )
 
   function unit() : F
   {
-    F(None, false, false, 0, zero_map())
-  }
-
-  function add_fns(f: FullMap<Base.M, nat>, g: FullMap<Base.M, nat>) : FullMap<Base.M, nat> {
-    imap b | true :: f[b] + g[b]
+    F(exc_unit(), exc_unit(), exc_unit(), 0, agn_unit())
   }
 
   function dot(a: F, b: F) : F
   {
-    if a.F? && b.F?
-      && !(a.central.CentralState? && b.central.CentralState?)
-      && !(a.exc_pending && b.exc_pending)
-      && !(a.exc_taken && b.exc_taken)
-    then
-      F(
-        if a.central.CentralState? then a.central else b.central,
-        a.exc_pending || b.exc_pending,
-        a.exc_taken || b.exc_taken,
+    F(
+        exc_dot(a.fields, b.fields),
+        exc_dot(a.exc_pending, b.exc_pending),
+        exc_dot(a.exc_taken, b.exc_taken),
         a.shared_pending_handles + b.shared_pending_handles,
-        add_fns(a.shared_taken_handles, b.shared_taken_handles))
-    else
-      Bot
+        agn_dot(a.shared_taken_handles, b.shared_taken_handles)
+    )
   }
 
   /* Validity predicate */
 
-  predicate P(f: F) {
-    && f != Bot
-    && f.central.CentralState?
-    && f.central.rc == f.shared_pending_handles + f.shared_taken_handles[f.central.held_value]
-    && (!f.central.exc ==> !f.exc_pending && !f.exc_taken)
-    && (f.central.exc ==> (f.exc_pending || f.exc_taken)
-                       && !(f.exc_pending && f.exc_taken))
-    && (f.exc_taken ==> forall y :: f.shared_taken_handles[y] == 0)
-    && (forall y :: f.shared_taken_handles[y] != 0 ==> f.central.held_value == y)
+  function agn_count<T>(x: Agn<T>): nat {
+      if x.Have? then x.n else 0
   }
 
-  predicate V(a: F) {
-    exists p :: P(dot(a, p))
+  predicate Inv(f: F) {
+    && exc_valid(f.fields)
+    && exc_valid(f.exc_pending)
+    && exc_valid(f.exc_taken)
+    && agn_valid(f.shared_taken_handles)
+
+    && f.fields.ExcOne?
+    && f.fields.t.rc == f.shared_pending_handles + agn_count(f.shared_taken_handles)
+    && (!f.fields.t.exc ==> !f.exc_pending.ExcOne? && !f.exc_taken.ExcOne?)
+    && (f.fields.t.exc ==> (f.exc_pending.ExcOne? || f.exc_taken.ExcOne?)
+                       && !(f.exc_pending.ExcOne? && f.exc_taken.ExcOne?))
+    && (f.exc_taken.ExcOne? ==> f.shared_taken_handles == Zero)
+    && (f.shared_taken_handles.Have? ==> f.shared_taken_handles.t == f.fields.t.x)
   }
 
-  /* Interpretation function */
+  /* Storage function */
 
-  // I_defined(f) means I(f) != bot
-  predicate I_defined(f: F) {
-    f == unit() || P(f)
-  }
-
-  function I(f: F) : Base.M
-  requires I_defined(f)
+  function Storage(f: F) : B
+  requires Inv(f)
   {
-    if f == unit() then
-      Base.unit()
-    else if f.exc_taken then
-      Base.unit()
+    if f.exc_taken.ExcOne? then
+        ExcEmpty
     else
-      f.central.held_value
+        ExcOne(f.fields.t.x)
   }
 
-  /* Transitions predicate */
-
-  predicate transitions(a: F, b: F) {
-    forall p :: I_defined(dot(a, p)) ==>
-        I_defined(dot(b, p)) && I(dot(a, p)) == I(dot(b, p))
-  }
-
-  /* TPCM properties */
+  /* PCM properties */
 
   lemma commutative(x: F, y: F)
   ensures dot(x, y) == dot(y, x)
   {
     if dot(x, y).F? {
-      assert dot(x, y).central == dot(y, x).central;
+      assert dot(x, y).fields == dot(y, x).fields;
       assert dot(x, y).exc_pending == dot(y, x).exc_pending;
       assert dot(x, y).exc_taken == dot(y, x).exc_taken;
       assert dot(x, y).shared_pending_handles == dot(y, x).shared_pending_handles;
@@ -116,7 +168,7 @@ module RWLock {
   ensures dot(x, dot(y, z)) == dot(dot(x, y), z)
   {
     if dot(x, dot(y, z)).F? {
-      assert dot(x, dot(y, z)).central == dot(dot(x, y), z).central;
+      assert dot(x, dot(y, z)).fields == dot(dot(x, y), z).fields;
       assert dot(x, dot(y, z)).exc_pending == dot(dot(x, y), z).exc_pending;
       assert dot(x, dot(y, z)).exc_taken == dot(dot(x, y), z).exc_taken;
       assert dot(x, dot(y, z)).shared_pending_handles == dot(dot(x, y), z).shared_pending_handles;
@@ -129,301 +181,144 @@ module RWLock {
   {
   }
 
-  lemma valid_monotonic(a: F, b: F)
-  requires V(dot(a, b))
-  ensures V(a)
+  /* Derived operators */
+
+  predicate exchange(p1: F, p2: F, b1: B, b2: B) {
+    forall q :: Inv(dot(p1, q)) ==>
+        && Inv(dot(p2, q))
+        && base_V(base_dot(Storage(dot(p1, q)), b1))
+        && base_dot(Storage(dot(p1, q)), b1) == base_dot(Storage(dot(p2, q)), b2)
+  }
+
+  predicate withdraw(p1: F, p2: F, b2: B) {
+    forall q :: Inv(dot(p1, q)) ==>
+        && Inv(dot(p2, q))
+        && Storage(dot(p1, q)) == base_dot(Storage(dot(p2, q)), b2)
+  }
+
+  predicate deposit(p1: F, p2: F, b1: B) {
+    forall q :: Inv(dot(p1, q)) ==>
+        && Inv(dot(p2, q))
+        && base_V(base_dot(Storage(dot(p1, q)), b1))
+        && base_dot(Storage(dot(p1, q)), b1) == Storage(dot(p2, q))
+  }
+
+  predicate transition(a: F, b: F) {
+    forall p :: Inv(dot(a, p)) ==>
+        Inv(dot(b, p)) && Storage(dot(a, p)) == Storage(dot(b, p))
+  }
+
+  predicate guards(f: F, m: B)
   {
-    var c :| P(dot(dot(a, b), c));
-    associative(a, b, c);
-    assert P(dot(a, dot(b, c)));
+    forall q :: Inv(dot(f, q)) ==>
+      exists z :: base_dot(m, z) == Storage(dot(f, q))
   }
 
-  lemma valid_unit()
-  ensures V(unit())
-  {
-    assert P(dot(unit(), Central(false, 0, Base.unit())));
+  /* Fields, ExcPending, ExcGuard, ShPending, ShGuard */
+
+  function Fields(exc: bool, rc: int, x: X) : F {
+    F(ExcOne(FieldsState(exc, rc, x)), ExcEmpty, ExcEmpty, 0, Zero)
   }
 
-  lemma reflexive(a: F)
-  ensures transitions(a, a)
-  {
-  }
+  const ExcPending : F := F(ExcEmpty, ExcOne(()), ExcEmpty, 0, Zero);
 
-  lemma transitive(a: F, b: F, c: F)
-  requires transitions(a, b)
-  requires transitions(b, c)
-  ensures transitions(a, c)
-  {
-  }
+  const ExcGuard : F := F(ExcEmpty, ExcEmpty, ExcOne(()), 0, Zero);
 
-  lemma monotonic(a: F, b: F, c: F)
-  requires transitions(a, b)
-  requires V(dot(a, c))
-  ensures V(dot(b, c))
-  ensures transitions(dot(a, c), dot(b, c))
-  {
-    assert V(dot(b, c)) by {
-      if dot(b, c) == unit() {
-        valid_unit();
-      } else {
-        var p :| I_defined(dot(dot(a, c), p));
-        associative(a, c, p);
-        associative(b, c, p);
-        assert I_defined(dot(dot(b, c), p));
-      }
-    }
-    assert transitions(dot(a, c), dot(b, c)) by {
-      forall p | I_defined(dot(dot(a, c), p))
-      ensures I_defined(dot(dot(b, c), p)) && I(dot(dot(a, c), p)) == I(dot(dot(b, c), p))
-      {
-        associative(a, c, p);
-        associative(b, c, p);
-      }
-    }
-  }
+  const ShPending : F := F(ExcEmpty, ExcEmpty, ExcEmpty, 1, Zero);
 
-  /* Central, ExcPending, ExcGuard, ShPending, ShGuard */
-
-  function Central(exc: bool, rc: nat, x: Base.M) : F {
-    F(CentralState(exc, rc, x), false, false, 0, zero_map())
-  }
-
-  const ExcPending : F := F(None, true, false, 0, zero_map());
-
-  const ExcGuard : F := F(None, false, true, 0, zero_map());
-
-  function unit_fn(elem: Base.M) : FullMap<Base.M, nat> {
-    imap b | true :: (if elem == b then 1 else 0)
-  }
-
-  const ShPending : F := F(None, false, false, 1, zero_map());
-
-  function ShGuard(elem: Base.M) : F {
-    F(None, false, false, 0, unit_fn(elem))
-  }
-
-  /* TPCM Extension properties */
-
-  lemma valid_domain(f: F)
-  requires I_defined(f)
-  ensures V(f)
-  {
-    if f != unit() {
-      dot_unit(f);
-      assert P(dot(f, unit()));
-      assert V(f);
-    } else {
-      assert P(dot(f, Central(false, 0, Base.unit())));
-    }
-  }
-
-  lemma extension_unit(f: F)
-  ensures I_defined(unit())
-  ensures I(unit()) == Base.unit()
-  {
-  }
-
-  lemma respects_transitions(f: F, f': F)
-  requires I_defined(f) && transitions(f, f')
-  ensures I_defined(f')
-  ensures Base.transitions(I(f), I(f'))
-  {
-    dot_unit(f);
-    assert I_defined(dot(f, unit()));
-    assert I_defined(dot(f', unit()));
-    dot_unit(f');
-    assert I_defined(f');
-    assert Base.transitions(I(f), I(f'));
+  function ShGuard(elem: X) : F {
+    F(ExcEmpty, ExcEmpty, ExcEmpty, 0, Have(elem, 1))
   }
 
   /* RwLock-Init */
 
-  lemma RwLockInit(x: Base.M)
-  ensures V(Central(false, 0, x))
+  lemma RwLockInit(x: X)
+  ensures Inv(Fields(false, 0, x))
   {
-    assert P(dot(Central(false, 0, x), unit()));
   }
 
   /* RwLock-Exc-Begin */
 
-  lemma RwLockExcBegin(rc: nat, x: Base.M)
-  ensures transitions(
-      Central(false, rc, x),
-      dot(Central(true, rc, x), ExcPending)
+  lemma RwLockExcBegin(rc: nat, x: X)
+  ensures transition(
+      Fields(false, rc, x),
+      dot(Fields(true, rc, x), ExcPending)
     )
   {
   }
 
   /* RwLock-Exc-Acquire */
 
-  predicate ExtExchangeCondition(f: F, m: Base.M, f': F, m': Base.M)
-  {
-    forall p :: I_defined(dot(f, p)) && Base.V(Base.dot(m, I(dot(f, p)))) ==>
-      I_defined(dot(f', p)) &&
-        Base.transitions(Base.dot(m, I(dot(f, p))), Base.dot(m', I(dot(f', p))))
-  }
-
-  lemma RwLockExcAcquire(exc: bool, x: Base.M)
-  ensures ExtExchangeCondition(
-      dot(Central(exc, 0, x), ExcPending),
-      Base.unit(),
-      dot(Central(exc, 0, x), ExcGuard),
-      x
+  lemma RwLockExcAcquire(exc: bool, x: X)
+  ensures withdraw(
+      dot(Fields(exc, 0, x), ExcPending),
+      dot(Fields(exc, 0, x), ExcGuard),
+      ExcOne(x)
     )
   {
-    var f := dot(Central(exc, 0, x), ExcPending);
-    var m := Base.unit();
-    var f' := dot(Central(exc, 0, x), ExcGuard);
-    var m' := x;
-    forall p | I_defined(dot(f, p)) && Base.V(Base.dot(m, I(dot(f, p))))
-    ensures I_defined(dot(f', p))
-    ensures Base.transitions(Base.dot(m, I(dot(f, p))), Base.dot(m', I(dot(f', p))))
-    {
-      assert m == I(dot(f', p));
-      assert m' == I(dot(f, p));
-      Base.commutative(m, m');
-      assert Base.dot(m, I(dot(f, p))) == Base.dot(m', I(dot(f', p)));
-    }
   }
 
   /* RwLock-Exc-Release */
 
-  lemma RwLockExcRelease(exc: bool, rc: nat, x: Base.M, y: Base.M)
-  ensures ExtExchangeCondition(
-      dot(Central(exc, rc, y), ExcGuard),
-      x,
-      Central(false, rc, x),
-      Base.unit()
+  lemma RwLockExcRelease(exc: bool, rc: nat, x: X, y: X)
+  ensures deposit(
+      dot(Fields(exc, rc, y), ExcGuard),
+      Fields(false, rc, x),
+      ExcOne(x)
     )
   {
-    var f := dot(Central(exc, rc, y), ExcGuard);
-    var m := x;
-    var f' := Central(false, rc, x);
-    var m' := Base.unit();
-    forall p | I_defined(dot(f, p)) && Base.V(Base.dot(m, I(dot(f, p))))
-    ensures I_defined(dot(f', p))
-    ensures Base.transitions(Base.dot(m, I(dot(f, p))), Base.dot(m', I(dot(f', p))))
-    {
-      assert forall b :: dot(f',p).shared_taken_handles[b] == dot(f,p).shared_taken_handles[b];
-
-      assert m == I(dot(f', p));
-      assert m' == I(dot(f, p));
-      Base.commutative(m, m');
-      assert Base.dot(m, I(dot(f, p))) == Base.dot(m', I(dot(f', p)));
-    }
   }
 
   /* RwLock-Shared-Begin */
 
-  lemma RwLockSharedBegin(exc: bool, rc: nat, x: Base.M)
-  ensures transitions(
-      Central(exc, rc, x),
-      dot(Central(exc, rc + 1, x), ShPending)
+  lemma RwLockSharedBegin(exc: bool, rc: nat, x: X)
+  ensures transition(
+      Fields(exc, rc, x),
+      dot(Fields(exc, rc + 1, x), ShPending)
     )
   {
-    var a := Central(exc, rc, x);
-    var b := dot(Central(exc, rc + 1, x), ShPending);
-    forall p | I_defined(dot(a, p))
-    ensures I_defined(dot(b, p))
-    ensures I(dot(a, p)) == I(dot(b, p))
-    {
-      assert forall y :: dot(b,p).shared_taken_handles[y] == dot(a,p).shared_taken_handles[y];
-    }
   }
 
   /* RwLock-Shared-Acquire */
 
-  lemma RwLockSharedAcquire(exc: bool, rc: nat, x: Base.M)
-  ensures transitions(
-      dot(Central(false, rc, x), ShPending),
-      dot(Central(false, rc, x), ShGuard(x))
+  lemma RwLockSharedAcquire(exc: bool, rc: nat, x: X)
+  ensures transition(
+      dot(Fields(false, rc, x), ShPending),
+      dot(Fields(false, rc, x), ShGuard(x))
     )
   {
-    var a := dot(Central(false, rc, x), ShPending);
-    var b := dot(Central(false, rc, x), ShGuard(x));
-    forall p | I_defined(dot(a, p))
-    ensures I_defined(dot(b, p))
-    ensures I(dot(a, p)) == I(dot(b, p))
-    {
-      assert forall y :: y != x ==>
-        dot(b,p).shared_taken_handles[y] == dot(a,p).shared_taken_handles[y];
-    }
   }
 
   /* RwLock-Shared-Release */
 
-  lemma RwLockSharedRelease(exc: bool, rc: nat, x: Base.M, y: Base.M)
-  requires V(dot(Central(exc, rc, x), ShGuard(y)))
-  ensures rc >= 1
-  ensures transitions(
-      dot(Central(exc, rc, x), ShGuard(y)),
-      Central(exc, rc - 1, x)
+  lemma RwLockSharedRelease(exc: bool, rc: nat, x: X, y: X)
+  ensures transition(
+      dot(Fields(exc, rc, x), ShGuard(y)),
+      Fields(exc, rc - 1, x)
     )
   {
-    assert rc >= 1 by {
-      var p :| P(dot(dot(Central(exc, rc, x), ShGuard(y)), p));
-      assert dot(dot(Central(exc, rc, x), ShGuard(y)), p).shared_taken_handles[y] >= 1;
-      assert x == y;
-    }
-
-    var a := dot(Central(exc, rc, x), ShGuard(y));
-    var b := Central(exc, rc - 1, x);
-    forall p | I_defined(dot(a, p))
-    ensures I_defined(dot(b, p)) && I(dot(a, p)) == I(dot(b, p))
-    {
-      var f := dot(a, p);
-      var f' := dot(b, p);
-      assert f.shared_taken_handles[y] > 0;
-      assert y == f.central.held_value;
-      assert forall b :: b != f.central.held_value ==>
-          f'.shared_taken_handles[b] == f.shared_taken_handles[b];
-    }
   }
 
   /* RwLock-Shared-Retry */
 
-  lemma RwLockSharedRetry(exc: bool, rc: nat, x: Base.M)
-  requires V(dot(Central(exc, rc, x), ShPending))
-  ensures rc >= 1
-  ensures transitions(
-      dot(Central(exc, rc, x), ShPending),
-      Central(exc, rc - 1, x)
+  lemma RwLockSharedRetry(exc: bool, rc: nat, x: X)
+  ensures transition(
+      dot(Fields(exc, rc, x), ShPending),
+      Fields(exc, rc - 1, x)
     )
   {
-    assert rc >= 1;
-
-    var a := dot(Central(exc, rc, x), ShPending);
-    var b := Central(exc, rc - 1, x);
-    forall p | I_defined(dot(a, p))
-    ensures I_defined(dot(b, p)) && I(dot(a, p)) == I(dot(b, p))
-    {
-      var f := dot(a, p);
-      var f' := dot(b, p);
-      assert forall b :: b != f.central.held_value ==>
-          f'.shared_taken_handles[b] == f.shared_taken_handles[b];
-    }
   }
 
   /* RwLock-Shared-Borrow */
 
-  predicate BorrowBackCondition(f: F, m: Base.M)
+  lemma RwLockSharedGuards(x: X)
+  ensures guards(ShGuard(x), ExcOne(x))
   {
-    forall p :: I_defined(dot(f, p)) ==>
-      exists z :: Base.dot(m, z) == I(dot(f, p))
-  }
-
-  lemma RwLockSharedBorrow(x: Base.M)
-  ensures BorrowBackCondition(ShGuard(x), x)
-  {
-    var f := ShGuard(x);
-    forall p | I_defined(dot(f, p))
-    ensures exists z :: Base.dot(x, z) == I(dot(f, p))
+    forall q | Inv(dot(ShGuard(x), q)) ensures
+      exists z :: base_dot(ExcOne(x), z) == Storage(dot(ShGuard(x), q))
     {
-      assert dot(f, p).shared_taken_handles[x] >= 1;
-      assert x == I(dot(f, p));
-
-      Base.dot_unit(x);
-      assert Base.dot(x, Base.unit()) == I(dot(f, p));
+      var z := base_unit();
+      assert base_dot(ExcOne(x), z) == Storage(dot(ShGuard(x), q));
     }
   }
 }
